rename Semantics.realize → Semantics.models

Logic/Logic/Logic.lean
@@ -46,17 +46,17 @@ def System.hom [System F] {G : Type u} [LogicSymbol G] (F : G →L F) : System G
 /- Semantics of F -/
 
 class Semantics (F : Type u) [LogicSymbol F] (Struc : outParam (Type w → Type v)) where
-  realize : {M : Type w} → Struc M → F →L Prop
+  models : {M : Type w} → Struc M → F →L Prop
 
 namespace Semantics
 variable {Struc : Type w → Type v} [𝓢 : Semantics F Struc]
 
-def realizeTheory {M : Type w} (s : Struc M) (T : Set F) : Prop :=
-    ∀ ⦃f⦄, f ∈ T → realize s f
+def modelsTheory {M : Type w} (s : Struc M) (T : Set F) : Prop :=
+    ∀ ⦃f⦄, f ∈ T → models s f
 
-postfix:max " ⊧ₛ " => realize
+postfix:max " ⊧ₛ " => models
 
-infix:55 " ⊧ₛ* " => realizeTheory
+infix:55 " ⊧ₛ* " => modelsTheory
 
 def consequence (T : Set F) (f : F) : Prop :=
     ∀ (M : Type w) [Inhabited M] (s : Struc M), s ⊧ₛ* T → s ⊧ₛ f
@@ -76,32 +76,32 @@ lemma valid_neg_iff (f : F) : Valid (~f) ↔ ¬Satisfiable f := by simp[Valid, S
 
 lemma not_satisfiable_finset [DecidableEq F] (t : Finset F) :
     ¬Satisfiableₛ (t : Set F) ↔ Valid (t.image (~·)).disj :=
-  by simp[Satisfiableₛ, realizeTheory, Valid, Finset.map_disj]
+  by simp[Satisfiableₛ, modelsTheory, Valid, Finset.map_disj]
 
-lemma realizeTheory_of_subset {T U : Set F} {s : Struc M} (h : s ⊧ₛ* U) (ss : T ⊆ U) : s ⊧ₛ* T :=
+lemma modelsTheory_of_subset {T U : Set F} {s : Struc M} (h : s ⊧ₛ* U) (ss : T ⊆ U) : s ⊧ₛ* T :=
   fun _ hf => h (ss hf)
 
-@[simp] lemma realizeTheoryEmpty {s : Struc M} : s ⊧ₛ* (∅ : Set F) := fun p => by simp
+@[simp] lemma modelsTheoryEmpty {s : Struc M} : s ⊧ₛ* (∅ : Set F) := fun p => by simp
 
-@[simp] lemma realizeTheory_insert {T : Set F} {f : F} {s : Struc M} :
+@[simp] lemma modelsTheory_insert {T : Set F} {f : F} {s : Struc M} :
     s ⊧ₛ* insert f T ↔ s ⊧ₛ f ∧ s ⊧ₛ* T := by
-  simp[realizeTheory]
+  simp[modelsTheory]
 
-@[simp] lemma realizeTheory_union {T U : Set F} {s : Struc M} :
+@[simp] lemma modelsTheory_union {T U : Set F} {s : Struc M} :
     s ⊧ₛ* T ∪ U ↔ s ⊧ₛ* T ∧ s ⊧ₛ* U := by
-  simp[realizeTheory]
+  simp[modelsTheory]
   exact
   ⟨fun h => ⟨fun f hf => h (Or.inl hf), fun f hf => h (Or.inr hf)⟩,
    by rintro ⟨h₁, h₂⟩ f (h | h); exact h₁ h; exact h₂ h⟩
 
-@[simp] lemma realizeTheory_image {f : α → F} {A : Set α} {s : Struc M} :
-    s ⊧ₛ* f '' A ↔ ∀ i ∈ A, s ⊧ₛ (f i) := by simp[realizeTheory]
+@[simp] lemma modelsTheory_image {f : α → F} {A : Set α} {s : Struc M} :
+    s ⊧ₛ* f '' A ↔ ∀ i ∈ A, s ⊧ₛ (f i) := by simp[modelsTheory]
 
-@[simp] lemma realizeTheory_range {f : α → F} {s : Struc M} :
-    s ⊧ₛ* Set.range f ↔ ∀ i, s ⊧ₛ (f i) := by simp[realizeTheory]
+@[simp] lemma modelsTheory_range {f : α → F} {s : Struc M} :
+    s ⊧ₛ* Set.range f ↔ ∀ i, s ⊧ₛ (f i) := by simp[modelsTheory]
 
 lemma satisfiableₛ_of_subset {T U : Set F} (h : Satisfiableₛ U) (ss : T ⊆ U) : Satisfiableₛ T :=
-  by rcases h with ⟨M, i, s, h⟩; exact ⟨M, i, s, realizeTheory_of_subset h ss⟩
+  by rcases h with ⟨M, i, s, h⟩; exact ⟨M, i, s, modelsTheory_of_subset h ss⟩
 
 lemma consequence_iff {T : Set F} {f : F} : T ⊨ f ↔ ¬Satisfiableₛ (insert (~f) T) := by
   simp[consequence, Satisfiableₛ]; constructor
@@ -140,11 +140,11 @@ lemma consistent_of_model {T : Set F}
 lemma consistent_of_satisfiable {T : Set F} : Semantics.Satisfiableₛ T → System.Consistent T := by
   rintro ⟨M, _, s, h⟩; exact consistent_of_model h
 
-lemma realize_of_proof {T : Set F} {f} (h : s ⊧ₛ* T) (b : T ⊢ f) : s ⊧ₛ f :=
+lemma models_of_proof {T : Set F} {f} (h : s ⊧ₛ* T) (b : T ⊢ f) : s ⊧ₛ f :=
   Sound.sound b M s h
 
-lemma realizeTheory_of_proofTheory {T U : Set F} (h : s ⊧ₛ* T) (b : T ⊢* U) : s ⊧ₛ* U :=
-  fun _ hf => realize_of_proof h (b hf)
+lemma modelsTheory_of_proofTheory {T U : Set F} (h : s ⊧ₛ* T) (b : T ⊢* U) : s ⊧ₛ* U :=
+  fun _ hf => models_of_proof h (b hf)
 
 end Sound
 
